#+title: Ec Vector Spaces
#+author: Jackson Mowry
#+date: Sun Oct 27 10:38:59 2024
#+options: \n:t toc:nil

* 6
The set V = {(x,y,z) | x,y,z are integers}, with regular component addition and scalar multiplication as the operations
1. ku \in V (Axiom 6)
   - Scalar multiples do not have to be integers \therefore{} ku \notin{} V
   - $u = (1,1,1), k = 4.5 \therefore ku = (4.5,4.5,4.5) \notin{} V$

* 7
The set V of all continuous functions that are differentiable on (-\inf(), \inf{})
1. u + v \in V
   - Both u and v are continuous and differentiable, u+v must also be continuous and differentiable (as the sum of continuous and differentiable functions respectively)
   - u + v \in V
2. u + v = v + u
   - Function addition is known to be commutative
   - Therefore u + v = v + u
3. u + (v + w) = (u + v) + w
   - Function addition is known to be associative
   - Therefore u + (v + w) = (u + v) + w
4. There exists a zero 0 \overrightarrow{0} such that 0 + u = u + 0 = u
   - The zero function f(x) = 0 for all x is continuous and differentiable, thus the zero vector is in V
5. For each u in V, there exists -u such that u + -u = 0
   - If a function f is continuous and differentiable, then -f must also be continuous and differentiable, thus -f \in V
6. ku \in V
   - If u is continuous and differentiable, then ku is continuous (since scalar multiples of continuous functions are continuous) and differentiable (since scalar multiples of differentiable functions are differentiable)
   - \therefore{} ku \in V
7. k(u + v) = ku + kv
   - This follows the basic properties of scalar multiplication and function addition
   - \therefore{} this property holds for our vector space
8. (k+m)u = ku + mu
   - This is the same property as scalar multiplication
   - $(k+m)u$
   - $uk + um$
   - $ku + mu$
9. (km)u = k(mu)
   - This follows the same properties as scalar multiplication as proven above
10. 1 \times{} u = u
    - We can simply substitute the value 0 in for '1' in the original axiom
      - Or the zero function
    - This is treated as an addition of the identity
    - $f(x) + 0 = f(x)$
