% Created 2024-08-28 Wed 09:38
% Intended LaTeX compiler: pdflatex
\documentclass[11pt]{article}
\usepackage[utf8]{inputenc}
\usepackage[T1]{fontenc}
\usepackage{graphicx}
\usepackage{longtable}
\usepackage{wrapfig}
\usepackage{rotating}
\usepackage[normalem]{ulem}
\usepackage{amsmath}
\usepackage{amssymb}
\usepackage{capt-of}
\usepackage{hyperref}
\date{\today}
\title{One Four}
\hypersetup{
 pdfauthor={},
 pdftitle={One Four},
 pdfkeywords={},
 pdfsubject={},
 pdfcreator={Emacs 29.4 (Org mode 9.8)}, 
 pdflang={English}}
\begin{document}

\maketitle
\tableofcontents

\section{Properties}
\label{sec:org60f12b8}
\begin{enumerate}
\item A+B=B+A
\item A+(B+C)=(A+B)+C
\item (km)A=k(mA)
\item 1A=A
\item k(A+B)=kA+kB
\item (k+m)A=Ka+mA
\item A+0\textsubscript{m x n} = A
\item A+(-A) = 0
\item If kA = 0\textsubscript{m x n} then k = 0, or A = 0\textsubscript{m x n}
\end{enumerate}
\section{Matrix Mul Props}
\label{sec:org25f2274}
\begin{enumerate}
\item A(BC) = (AB)C
\item A(B+C) = AB+AC
\item (A+B)C=AC+BC
\item k(AB)=(kA)B=A(kB)
\end{enumerate}

AB \(\neq\) BA in general

\begin{verbatim}
A_{2x3}B_{3x2} -> 2x2
B_{3x2}A_{2x3} -> 3x3
\end{verbatim}
\section{Matrix Transpost Props}
\label{sec:org8feafb6}
\begin{enumerate}
\item (A\textsuperscript{T})\textsuperscript{T} = A
\item (A+B)\textsuperscript{T} = A\textsuperscript{T} + B\textsuperscript{T}
\item (kA)\textsuperscript{T} = k(A\textsuperscript{T})
\item (AB)\textsuperscript{T} = B\textsuperscript{T}A\textsuperscript{T}
\end{enumerate}
\end{document}
