#+title: Notes
* 2a.
\Sigma = {a,b,c}
R:      S \rightarrow{} A
        A \rightarrow{} AaB
        B \rightarrow{} b | C | \epsilon{}
        C \rightarrow{} CC | c | \epsilon{}

- Step 2 removing Epsilon Rules
  - Removing B \rightarrow{} \epsilon{}
    - S \rightarrow{} A
    - A \rightarrow{} AaB | Aa
    - B \rightarrow{} b | C
    - C \rightarrow{} CC | c | \epsilon{}
  - Removing C \rightarrow{} \epsilon{}
    - S \rightarrow{} A
    - A \rightarrow{} AaB | Aa
    - B \rightarrow{} b | C
    - C \rightarrow{} CC | c
* 3b.
\Sigma{} = {a,b,c}
R:
- S \rightarrow{} A | \epsilon{}
- A \rightarrow{} BC
- B \rightarrow{} BD | bb
- C \rightarrow{} CD | cc
- D \rightarrow{} B | C

Step 3 Removal of unit rules (remember we can have epsilon because the empty string is in the language)
- S \rightarrow{} *A* | \epsilon{}
- A \rightarrow{} BC
- B \rightarrow{} BD | bb
- C \rightarrow{} CD | cc
- *D \rightarrow{} B | C*

Removing S \rightarrow{} A
- S \rightarrow{} BC | \epsilon{}
- A \rightarrow{} BC
- B \rightarrow{} BD | bb
- C \rightarrow{} CD | cc
- D \rightarrow{} B | C

Removing B \rightarrow{} D
- S \rightarrow{} BC | \epsilon{}
- A \rightarrow{} BC
- B \rightarrow{} BD | bb
- C \rightarrow{} CD | cc
- D \rightarrow{} BD | bb | C

Removing D \rightarrow{} C
- S \rightarrow{} BC | \epsilon{}
- A \rightarrow{} BC
- B \rightarrow{} BD | bb
- C \rightarrow{} CD | cc
- D \rightarrow{} BD | bb | CD | cc

A is now redundent
